\documentclass[main.tex]{subfiles}

\begin{document}
\problem{Prove the trigonometric formula: 
$\cos{(\theta_1 - \theta_2)} = 
\cos\theta_1 \cos\theta_2 + \sin\theta_1 \sin\theta_2$.\\
(Hint: consider two unit vectors making angles $\theta_1$ and $\theta_2$ 
with the positive x-axis.)}

{

\tikz[scale=6] \coordinate (O) at (0,0);
\tikz[scale=6] \coordinate (A) at ($(O)!1 cm!-35:(0,1)$);
\tikz[scale=6] \coordinate (B) at ($(O)!1 cm!-65:(0,1)$);
\tikz[scale=6] \coordinate (i) at (1,0);
\tikz[scale=6] \coordinate (j) at (0,1);


Consider the unit vectors $\vec{A}$ and $\vec{B}$. These vectors make 
angles of $\theta_1$ and $\theta_2$, respectivley, with respect to the
positive x-axis (and the basis vector $\bi$)


\begin{figure}[h!]
    \centering
    \begin{tikzpicture}[scale=4]
    
		% Draw basis vectors
		\draw [i, ->] (O) -- (i);
		\draw [j, ->] (O) -- (j);
		
		\begin{scope}[thick]
			\draw [->, color=1] (O) -- (A);
			\draw [->, color=2] (O) -- (B);
		\end{scope}
		
		\pic [->, draw=1, "$\color{1}\theta_1$", angle eccentricity=1.5]
                {angle = i--O--A};
		\pic [->, draw=2, "\color{2}$\theta_2$", angle radius=40, 
              angle eccentricity=1.2]
              {angle = i--O--B};

    \end{tikzpicture}
    \caption{unit vectors $\vec{A}$ and $\vec{B}$}

\end{figure}


Considering just $\theta_1$, using the dot product we have 
\[\vec{A}\cdot\bi = |\vec{A}||\bi|\cos{\theta_1}.\] Which simplifies to
\[\vec{A}\cdot\bi = \cos{\theta_1},\] because both vectors are of unit length.
Similarly,
 \[\vec{B}\cdot\bi = \cos{\theta_2}.\]
Notice that the angle between $\vec{A}$ and $\vec{B}$ is $\theta_1 - \theta_2$.
(Certainly, at least in the case where $\theta_1 > \theta_2$.) By the same 
method as above we would find \[\vec{A}\cdot\vec{B} = \cos(\theta_1 - \theta_2)\]


\begin{figure}[h!]
    \centering
    \begin{tikzpicture}

		% Draw basis vectors
		\draw [i, ->] (O) -- (i);
		\draw [j, ->] (O) -- (j);
		
		\begin{scope}[thick]
			\draw [->, color=1] (O) -- (A);
		\end{scope}
		
		\begin{scope}[dashed]
			\draw[1!50!j] ($(O)!(A)!(i)$) -- 
							node[midway, right]{$\vec{A}\cdot\bj = \cos{(\frac{\pi}{2}-\theta_1)}$}
							(A);
			\draw[1!50!i] ($(O)!(A)!(j)$) -- 
							node[midway, above]{$\vec{A}\cdot\bi = \cos{\theta_1}$}
							(A);
		\end{scope}
		
		
		\pic [draw=1, "$\color{1}\theta_{1}$", angle eccentricity=2]
                {angle = i--O--A};

    \end{tikzpicture}
    \caption{unit vector $\vec{A}$}

\end{figure}

Let's turn our attention to focus on $\vec{A}$. We have observed that the angle
to $\bi$ is $\theta_1$. 
Notice that the angle between $\vec{A}$ and $\bj$ is $\frac{\pi}{2} - \theta_1$.
And $\cos{(\frac{\pi}{2} - \theta_1)} = \sin{\theta_1}$.
So, $\vec{A}\cdot\bj = \sin{\theta_1}$
Now consider that 
\begin{align*}
\vec{A} &= (\vec{A}\cdot\bi)\bi + (\vec{A}\cdot\bj)\bj\\
&= \cos{\theta_1}\bi + \sin{\theta_1}\bj,
\end{align*}
while
\begin{align*}
\vec{B} &= (\vec{B}\cdot\bi)\bi + (\vec{B}\cdot\bj)\bj\\
&= \cos{\theta_2}\bi + \sin{\theta_2}\bj.
\end{align*}
We can rewrite the dot product of $\vec{A}$ and $\vec{B}$
\begin{align*}
\vec{A}\cdot\vec{B} &= (\cos{\theta_1}\bi + \sin{\theta_1}\bj) \cdot
(\cos{\theta_2}\bi + \sin{\theta_2}\bj)\\
\begin{split}
&= 
\cos{\theta_1}\bi \cdot\cos{\theta_2}\bi 
+ \cos{\theta_1}\bi \cdot\sin{\theta_2}\bj
+\sin{\theta_1}\bj\cdot\cos{\theta_2}\bi 
+ \sin{\theta_1}\bj\cdot\sin{\theta_2}\bj
\end{split}\\
\begin{split}
&= 
(\cos{\theta_1}\cos{\theta_2})(\bi \cdot\bi)
+ (\cos{\theta_1}\sin{\theta_2})(\bi \cdot\bj)
+ (\sin{\theta_1}\cos{\theta_2})(\bj\cdot\bi)
+ (\sin{\theta_1}\sin{\theta_2})(\bj\cdot\bj).
\end{split}
\end{align*}
We can simplify this because $\bi\cdot\bi = |\bi|^2 = |\bj|^2 =\bj\cdot\bj = 1$ 
and $\bi\cdot\bj = 0$
\begin{align*}
\vec{A}\cdot\vec{B} &=  
\cos{\theta_1}\cos{\theta_2}
+ \sin{\theta_1}\sin{\theta_2}.
\end{align*}
Thus,\[
\cos{(\theta_1 - \theta_2)} = 
\cos{\theta_1}\cos{\theta_2}
+ \sin{\theta_1}\sin{\theta_2}.
\]

}


\end{document}

